cleanup, commenting, wip in ctreestheory. Proof of up-to bind for wbisim in progress

theories/CTreesTheory.v
@@ -1,4 +1,10 @@
-(* begin hide *)
+(*|
+==============================
+Equational Theory for [ctrees]
+==============================
+
+.. coq::none
+|*)
 From Coq Require Import
      Program
      Setoid
@@ -8,17 +14,41 @@ From Coq Require Import
 From Coinduction Require Import
 	   coinduction rel tactics.
 
+From RelationAlgebra Require Import
+     monoid
+     kat
+     kat_tac
+     prop
+     rel
+     srel
+     comparisons
+     rewriting
+     normalisation.
+
 From CTree Require Import
 	   Utils CTrees Shallow Trans Equ Bisim.
 
 Obligation Tactic := idtac.
-(* end hide *)
 
 Import CTree.
 Import CTreeNotations.
 Open Scope ctree.
 
 
+(*|
+Up-to [equ eq] bisimulations
+----------------------------
+We have proved in the module [Bisim] that [sbisim] and [wbisim] are closed under [equ eq].
+We prove here more generally that strong and weak bisimulation up-to [equ eq] are valid
+reasoning principles.
+
+Note: Should probably refactor things to prove this first and derive the particular case as
+a consequence.
+|*)
+
+(*|
+Definition of the enhancing function
+|*)
 Variant equ_clos_body {E X1 X2} (R : rel (ctree E X1) (ctree E X2)) : (rel (ctree E X1) (ctree E X2)) :=
   | Equ_clos : forall t t' u' u
                  (Equt : t ≅ t')
@@ -34,13 +64,19 @@ Next Obligation.
   apply LE; auto.
 Qed.
 
+(*|
+Sufficient condition to prove compatibility only over the simulation
+|*)
 Lemma equ_clos_sym {E X} : compat converse (@equ_clos E X X).
 Proof.
-  intros R t u EQ; inv EQ. 
-  apply Equ_clos with u' t'; intuition. 
+  intros R t u EQ; inv EQ.
+  apply Equ_clos with u' t'; intuition.
 Qed.
 
-Lemma equ_clos_t {E X} : @equ_clos E X X <= st.
+(*|
+Strong bisimulation up-to [equ] is valid
+|*)
+Lemma equ_clos_st {E X} : @equ_clos E X X <= st.
 Proof.
   apply Coinduction, by_Symmetry; [apply equ_clos_sym |].
   intros R t u EQ l t1 TR; inv EQ.
@@ -55,52 +91,77 @@ Proof.
   auto.
 Qed.
 
+(*|
+TODO: Can we afford to make [wtrans] opaque? If so, where?
+|*)
+Opaque wtrans.
+(*|
+Weak bisimulation up-to [equ] is valid
+|*)
+Lemma equ_clos_wt {E X} : @equ_clos E X X <= wt.
+Proof.
+  apply Coinduction, by_Symmetry; [apply equ_clos_sym |].
+  intros R t u EQ l t1 TR; inv EQ.
+  destruct HR as [F _]; cbn in *.
+  rewrite Equt in TR.
+  apply F in TR.
+  destruct TR as [? ? ?].
+  eexists.
+  rewrite <- Equu; eauto.
+  apply (f_Tf wb).
+  econstructor; intuition.
+  auto.
+Qed.
+
+(*|
+Up-to [bind] context bisimulations
+----------------------------------
+We have proved in the module [Equ] that up-to bind context is
+a valid enhancement to prove [equ].
+We now prove the same result, but for strong and weak bisimulation.
+|*)
+
 Section bind.
 
-  Section Concrete_Bind_ctx.
 
-    Context {E: Type -> Type} {X1 X2 Y1 Y2: Type}.
+(*|
+Specialization of [bind_ctx] to the [sbisim]-based closure we are
+looking for, and the proof of validity of the principle. 
+|*)
+   Section Sbisim_Bind_ctx.
 
-    (* specialisation to a function acting with [sbisim] on the bound value, and with the argument (pointwise) on the continuation *)
-    Program Definition bind_ctx_sbisim : mon (rel (ctree E Y1) (ctree E Y1)) :=
-      {|body := fun R => @bind_ctx E X1 X1 Y1 Y1 sbisim (pointwise eq R) |}.
+    Context {E: Type -> Type} {X Y: Type}.
+
+(*|
+Specialization of [bind_ctx] to a function acting with [sbisim] on the bound value,
+and with the argument (pointwise) on the continuation.
+|*)
+    Program Definition bind_ctx_sbisim : mon (rel (ctree E Y) (ctree E Y)) :=
+      {|body := fun R => @bind_ctx E X X Y Y sbisim (pointwise eq R) |}.
     Next Obligation.
       intros ?? H. apply leq_bind_ctx. intros ?? H' ?? H''.
       apply in_bind_ctx. apply H'. intros t t' HS. apply H, H'', HS.
     Qed.
 
-    (* this gives a valid up-to technique *)
-    Lemma bind_ctx_equ_t (SS : rel X1 X2) (RR : rel Y1 Y2): @bind_ctx_equ E _ _ _ _ SS <= t_equ RR.
+
+(*|
+Sufficient condition to exploit symmetry
+|*)
+    Lemma bind_ctx_sbisim_sym: compat converse bind_ctx_sbisim.
     Proof.
-      apply Coinduction. intros R. apply (leq_bind_ctx _).
-      intros x x' xx' k k' kk'.
-      step in xx'.
-      cbn; unfold observe; cbn.
-      destruct xx'.
-      - cbn in *.
-        generalize (kk' _ _ REL).
-        apply (fequ RR).
-        apply id_T.
-      - constructor; intros ?. apply (fTf_Tf (fequ _)).
-        apply in_bind_ctx. apply REL.
-        red; intros. apply (b_T (fequ _)), kk'; auto.
-      - constructor. intro a. apply (fTf_Tf (fequ _)).
-        apply in_bind_ctx. apply REL.
-        red; intros. apply (b_T (fequ _)), kk'; auto.
+      intro R. simpl. apply leq_bind_ctx. intros. apply in_bind_ctx.
+      symmetry; auto.
+      intros ? ? ->.
+      apply H0; auto.
     Qed.
 
-    Lemma bind_ctx_sym: compat converse bind_ctx_sbisim.
-    Proof. intro R. simpl. apply leq_bind_ctx. intros. apply in_bind_ctx.
-           symmetry; auto.
-           intros ? ? ->.
-           apply H0; auto.
-    Qed.
-
-    (* this gives a valid up-to technique *)
+(*|
+The resulting enhancing function gives a valid up-to technique
+|*)
     Lemma bind_ctx_sbisim_t : bind_ctx_sbisim <= st.
     Proof.
       apply Coinduction, by_Symmetry.
-      apply bind_ctx_sym.
+      apply bind_ctx_sbisim_sym.
       intros R. apply (leq_bind_ctx _).
       intros t1 t2 tt k1 k2 kk.
       step in tt; destruct tt as (F & B); cbn in *.
@@ -108,6 +169,69 @@ Section bind.
       apply trans_bind_inv in STEP as [(H & t' & STEP & EQ) | (v & STEPres & STEP)]; cbn in *.
       - apply F in STEP as [u' STEP EQ'].
         eexists.
+        apply trans_bind_l; eauto.
+        apply (fT_T equ_clos_st).
+        econstructor; [exact EQ | | reflexivity].
+        apply (fTf_Tf sb).
+        apply in_bind_ctx; auto.
+        intros ? ? ->.
+        apply (b_T sb).
+        apply kk; auto.
+      - apply F in STEPres as [u' STEPres EQ'].
+        pose proof (trans_val_inv _ _ _ STEPres) as EQ.
+        rewrite EQ in STEPres.
+        specialize (kk v v eq_refl) as [Fk Bk].
+        apply Fk in STEP as [u'' STEP EQ'']; cbn in *.
+        eexists.
+        eapply trans_bind_r; cbn in *; eauto.
+        eapply (id_T sb); cbn; auto.
+    Qed.
+
+   End Sbisim_Bind_ctx.
+
+   Section Wbisim_Bind_ctx.
+
+    Context {E: Type -> Type} {X Y: Type}.
+
+(*|
+Specialization of [bind_ctx] to a function acting with [sbisim] on the bound value,
+and with the argument (pointwise) on the continuation.
+|*)
+    Program Definition bind_ctx_wbisim :  mon (rel (ctree E Y) (ctree E Y)) :=
+      {|body := fun R => @bind_ctx E X X Y Y wbisim (pointwise eq R) |}.
+    Next Obligation.
+      intros ???? H. apply leq_bind_ctx. intros ?? H' ?? H''.
+      apply in_bind_ctx. apply H'. intros t t' HS. apply H0, H'', HS.
+    Qed.
+
+(*|
+Sufficient condition to exploit symmetry
+|*)
+    Lemma bind_ctx_wbisim_sym: compat converse bind_ctx_wbisim.
+    Proof.
+      intro R. simpl. apply leq_bind_ctx. intros. apply in_bind_ctx.
+      symmetry; auto.
+      intros ? ? ->.
+      apply H0; auto.
+    Qed.
+
+
+(*|
+The resulting enhancing function gives a valid up-to technique
+|*)
+    Lemma bind_ctx_wbisim_t : bind_ctx_wbisim <= wt.
+    Proof.
+      apply Coinduction, by_Symmetry.
+      apply bind_ctx_wbisim_sym.
+      intros R. apply (leq_bind_ctx _).
+      intros t1 t2 tt k1 k2 kk.
+      step in tt; destruct tt as (F & B); cbn in *.
+      cbn in *; intros l u STEP.
+      apply trans_bind_inv in STEP as [(H & t' & STEP & EQ) | (v & STEPres & STEP)]; cbn in *.
+      - apply F in STEP as [u' STEP EQ'].
+        eexists.
+        (* TODO: wtrans bind lemmas *)
+(*
         apply trans_bind_l; eauto.
         apply (fT_T equ_clos_t).
         econstructor; [exact EQ | | reflexivity].
@@ -125,14 +249,9 @@ Section bind.
         eapply trans_bind_r; cbn in *; eauto.
         eapply (id_T sb); cbn; auto.
     Qed.
+ *)
+        Admitted.
 
-    (* specialisation to a function acting with [sbisim] on the bound value, and with the argument (pointwise) on the continuation *)
-    Program Definition bind_ctx_wbisim {E X Y1 Y2}: mon (rel (ctree E Y1) (ctree E Y2)) :=
-      {|body := fun R => @bind_ctx E X X Y1 Y2 wbisim (pointwise eq R) |}.
-    Next Obligation.
-      intros ?????? H. apply leq_bind_ctx. intros ?? H' ?? H''.
-      apply in_bind_ctx. apply H'. intros t t' HS. apply H, H'', HS.
-    Qed.
 
     (* this gives a valid up-to technique *)
     (* research question: is there a meaningful way do deal with bind_ctx in general? *)
@@ -155,9 +274,7 @@ Section bind.
         red; intros. apply (b_T (fequ _)), kk'; auto.
     Qed.
 
-
-
-  End Concrete_Bind_ctx.
+  End Wbisim_Bind_ctx.
 
 
 End bind.
